# 1.3 Determining Limits Questions

[[Calculus and Vectors]]
[[1.3 Determining Limits]]

1. ## $\lim_{x \to 3} \frac{x-3}{x+3}$
	Try Substitution here.
		$$\frac{3-3}{3+3}=\frac{0}{6}=0$$
			$$\lim_{x \to 3}\frac{x-3}{x+3}=0$$
2. ## $\lim_{x \to 0} \frac{x^2+2x-3}{x^2+2}$
	Use Substitution in a problem like this.
		$$\frac{0+0-3}{0+2}=\frac{-3}{2}$$
			$$\lim_{x \to 0}\frac{x^2+2x-3}{x^2+2}=\frac{-3}{2}$$
3. ## $\lim_{x \to -2} \frac{2x^2+5x+2}{x^2-2x-8}$
	Substitution will yield $\frac{0}{0}$, which is inconclusive.
	Factoring will have to be used.
		$$\lim_{x \to -2}\frac{(2x+1)(x+2)}{(x-4)(x+2)}$$
			$$\lim_{x \to -2}\frac{2x+1}{x-4}$$
				$$\frac{2(-2)+1}{-2-4}$$
					$$\frac{-3}{-6}=\frac{1}{2}$$
						$$\lim_{x \to -2}\frac{(2x+1)(x+2)}{(x-4)(x+2)}=\frac{1}{2}$$
4. ## $\lim_{x \to \infty} 13^{-x}$
	Although seemingly difficult at first glance, only substitution is needed. Since $x$ approaches $-\infty$, we can tell that the answer will be $0$.
		$$\lim_{x \to -\infty}13^{-\infty}=13^{-\infty}=\frac{1}{13^\infty}=\frac{1}{\infty}=0$$
5. ## $\lim_{x \to 4} \frac{x-4}{\sqrt{x}-2}$
	Substitution will yield an inconclusive statement
		$$$\lim_{x \to 4} \frac{x-4}{\sqrt{x}-2}=\frac{4-4}{\sqrt{4}-2}=\frac{0}{2-2}=\frac{0}{0}$$
		Rationalize the denominator by multiplying by the conjugate $(\sqrt{x}+2)$.
			$$\lim_{x \to 4} \frac{x-4}{\sqrt{x}-2}=\lim_{x \to 4}\frac{(x-4)(\sqrt{x}+2)}{(\sqrt{x}-2)(\sqrt{x}+2)}$$
				$$\lim_{x \to 4}\frac{(x-4)(\sqrt{x}+2)}{x-4}$$
					$$\lim_{x \to 4}(\sqrt{x}+2)$$
						Now sub in 4 for $x$.
						$$\sqrt{4}+2$$
							$$2+2=4$$
								 $$\lim_{x \to 4} \frac{x-4}{\sqrt{x}-2}=4$$
6. ## $\lim_{x \to 1} \frac{x^3-1}{x^3-x^2-4x+4}$
	Substitution will lead to inconclusive statement, $\frac{0}{0}$, take my word for it.\
	Factoring can be used for this.
		$$\lim_{x \to 1} \frac{x^3-1}{x^3-x^2-4x+4}=\lim_{x \to 1}\frac{(x-1)(x^2+x+1)}{(x-1)(x+2)(x+2)}=\lim_{x \to 1}\frac{x^2+x+1}{(x+2)(x-2)}$$
			Now substitution can be used.
			$$\frac{(1)^2+(1)+1}{(1+2)(1-2)}=\frac{3}{-3}=-1$$
				$$\lim_{x \to 1} \frac{x^3-1}{x^3-x^2-4x+4}=-1$$


