# 1.4 First Principles Questions
[[Calculus and Vectors]]\
[[1.4 Using First Principles to Determine Equation of a Tangent]]

### 1. Find the slope of the tangent line at point $(3,-9)$ on the curve $f(x)=3x-2x^2$
##### To find the slope of the tangent line at point $(3,-9)$, we will use first principles.
#### $$m=\lim_{h \to 0}\frac{f(a+h)-f(a)}{h}$$
$$m=\lim_{h \to 0}\frac{f(3+h)-f(3)}{h}$$
		$$m=\lim_{h \to 0}\frac{[9+3h-2(9+6h+h^2)]-[-9]}{h}$$
			$$m=\lim_{h \to 0}\frac{9+3h-18-12h-2h^2+9}{h}$$
				$$m=\lim_{h \to 0}\frac{-2h^2-9h}{h}$$
					$$m=\lim_{h \to 0}(-2h-9)$$
						$$m=-9$$

The slope of the tangent line at point (3,-9) on the curve $f(x)=3x-2x^2$ is $-9$.

### 2. Find the derivative of the function $f(x)=x^2+5x-7$ using First Principles
#### $$f'(x)=\lim_{h \to 0}\frac{f(x+h)-f(x)}{h}$$
$$f'(x)=\lim_{h \to 0}\frac{[(x+h)^2+5(x+h)-7]-[x^2+5x-7]}{h}$$
	$$f'(x)=\lim_{h \to 0}\frac{x^2+2xh+h^2+5x+5h-7-x^2-5x+7}{h}$$
		$$f'(x)=\lim_{h \to 0}\frac{h^2+2xh+5h}{h}$$
			$$f'(x)=\lim_{h \to 0}(h+2x+5)$$
				$$f'(x)=2x+5$$
The derivative of the function $f(x)=x^2+5x-7$ using First Principles is $2x+5$.

### 3. Find the sequation of the tangent line at point (-2,-3) on the curve $f(x)=x^2+3x-1$.

The Point is (-2,-3).
##### **First**, we must find the slope using first principles.

#### $$m=\lim_{h \to 0}\frac{f(a+h)-f(a)}{h}$$
$$m=\lim_{h \to 0}\frac{[(-2+h)^2+3(-2+h)-1]-[(-2)^2+3(-2)-1]}{h}$$
	$$m=\lim_{h \to 0}\frac{[4-4h+h^2-6+3h-1]-[-3]}{h}$$
		$$m=\lim_{h \to 0}\frac{h^2-1h}{h}$$
			$$m=\lim_{h \to 0}(h-1)$$
				$$m=-1$$
###### **Second,** we use the slope, $-1$, to find the equation of the line.
#### $$y=m(x-x_1)+y_1$$
$$y=(-1)[x-(-2)]+(-3)$$
	$$y=-(x+2)-3$$
		$$y=-x-2-3$$
			$$y=-x-5$$
The equation of the tangent line at point $(-2,-3)$ on the curve $f(x)=x^2+3x-1$ is $y=-x-5$.

### Bonus!! 
Using a graphing app, graph the function $f(x)=x^2+3x-1$ and the tangent line $y=-x-5$ from the previous question.

What do you notice?
![[1.4 Bonus Question.png]]
The tangent line $y=-x-5$ touches the graph of $f(x)=x^2+3x-1$ at the point $(-2,-3)$.
