# Determining Equation of a Tangent
[[Calculus and Vectors]]\
[[1.4 Using First Principles to Determine Equation of a Tangent Questions]]

The point $P(1,3)$ lies on the curve $f(x)=2x+x^2$
![[Tangent Point.png]]

 If $Q$ is the point $(x,2x+x^2)$, find the coordinates of point $Q$ for the following values of $x$. Unlike the secant method for finding the approximate instantaneous rate of change along a curve, this method is more precise, albeit more complicated.

 1. ### Complete a table for these values of $x$.

| x     | $f(x)=2x+x^2$                         | $Q(x,2x+x^2)$      |
| ----- | ------------------------------------- | ------------------ |
| 2     | $f(2)=2(2)+(2)^2=8$                   | $(2,8)$            |
| 1.5   | $f(1.5)=2(1.5)+(1.5)^2=5.25$          | $(1.5,5.25)$       |
| 1.1   | $f(1.1)=2(1.1)+(1.1)^2=3.41$          | $(1.1,3.41)$       |
| 1.01  | $f(1.01)=2(1.01)+(1.01)^2=3.041$      | $(1.01,3.0401)$    |
| 1.001 | $f(1.001)=2(1.001)+(1.001)^2=3.0041$  | $(1.001,3.004001)$ |
| 0.999 | $f(0.999)=2(0.999)+(0.999)^2=2.99601$ | $(0.999,2.996001)$ |
| 0.99  | $f(0.99)=2(0.99)+(0.99)^2=2.9601$     | $(0.99,2.9601)$    |
| 0.9   | $f(0.9)=2(0.9)+(0.9)^2=2.61$          | $(0.9,2.61)$       |
| 0.5   | $f(0.5)=2(0.5)+(0.5)^2=1.25$          | $(0.5,1.25)$       |
| 0     | $f(0)=2(0)+(0)^2=0$                   | $(0,0)$                   |

2. ### Find the slope of the secant line $PQ$ for the following values of $x$. Complete the following table using slope formula, $m=\frac{y_2-y_1}{x_2-x_1}$

Average Rate of Change Table

| $P(x_1,y_1)$ | $Q(x_2,y_2)$       | Average rate of Change $m=\frac{y_2-y_1}{x_2-x_1}$ |
| ------------ | ------------------ | -------------------------------------------------- |
| $(1,3)$      | $(2,8)$            | 5                                                  |
| $(1,3)$      | $(1.5,5.25)$       | 4.5                                                |
| $(1,3)$      | $(1.1,3.41)$       | 4.1                                                   |
| $(1,3)$      | $(1.01,3.0401)$    | 4.0                                                   |
| $(1,3)$      | $(1.001,3.004001)$ | 4.001                                                   |
| $(1,3)$      | $(0.999,2.997001)$ | 3.999                                                   |
| $(1,3)$      | $(0.99,2.9601)$    | 3.99                                                   |
| $(1,3)$      | $(0.9,2.61)$       | 3.9                                                   |
| $(1,3)$      | $(0.5,1.25)$       | 3.5                                                   |
| $(1,3)$      | $(0,0)$            | 3                                                   |


3. ### Using these results, find the slope of the tangent line to the curve at $P(1,3)$

From the table, the conclusion can be drawn that as the value $x=1$ is approached, in this case using 1.001 and 0.999 and giving the results 4.001 and 3.999 respectively, that the value of the slope of that line is converging on the value of 4.\
	Therefore, the value of the slope of the tangent line to the curve $P(1,3)$ is 4.

4. ### Using the slope of this tangent line, 4,  find the equation of the tangent line to the curve $P(1,3)$

The equation of a line is $$y=m(x-x_1)+y_1$$
The slope is 4 and the point is at $(1,3)$.
$$y=m(x-x_1)+y_1$$
	$$y=4(x-1)+3$$
		$$y=4x-4+3$$
			$$y=4x-1$$
			
## First Principles
#### $$ Derivative=f'(x)=y'=\lim_{h \to 0}\frac{f(x+h)-f(x)}{h}$$

Example: Find the derivative of $f'(x)=2x-x^2$ using first principles.

$$f'(x)=\lim_{h \to 0}\frac{f(x+h)-f(x)}{h}$$
	$$f'(x)=\lim_{h \to 0}\frac{[2(x+h)-(x+h)^2]-[2x-x^2]}{h}$$
		$$f'(x)=\lim_{h \to 0}\frac{[2x+2h-x^2-2xh-h^2]-[2x-x^2]}{h}$$
			$$f'(x)=\lim_{h \to 0}\frac{2x+2h-x^2-2xh-h^2-2x-x^2}{h}$$
				$$f'(x)=\lim_{h \to 0}\frac{2h-2xh-h^2}{h}$$
					$$f'(x)=\lim_{h \to 0}\frac{h(2-2x-h)}{h}$$
						$$f'(x)=\lim_{h \to 0}(2-2x-h)$$
							$$f'(x)=2-2x-0$$
								$$f'(x)=2-2x$$

### Now, try to find the derivative of the function $f(x)=2x^2-3x+1$ using First Principles.

$$f'(x)=\lim_{h \to 0}\frac{f(x+h)-f(x)}{h}$$
	$$f'(x)=\lim_{h \to 0}\frac{[2(x+h)^2-3(x+h)+1]-[2x^2-3x+1]}{h}$$
		$$f'(x)=\lim_{h \to 0}\frac{[2(x^2+2xh+h^2)-3x-3h+1]-[2x^2-3x+1]}{h}$$
			$$f'(x)=\lim_{h \to 0}\frac{2x^2+4xh+2h^2-3x-3h+1-2x^2+3x-1}{h}$$
				$$f'(x)=\lim_{h \to 0}\frac{2h^2+4xh-3h}{h}$$
					$$f'(x)=\lim_{h \to 0}(2h+4x-3)$$
						$$f'(x)=4x-3$$
							The derivative of the function $f(x)=2x^2-3x+1$	using first principles is $4x-3$.		

### Find the slope of the tangent line at point (1,3) on the curve $f(x)=2x+x^2$
	
$$m=\lim_{h \to 0}\frac{f(1+h)-f(1)}{h}$$
	$$m=\lim_{h \to 0}\frac{[2(1+h)+(1+h)^2]âˆ’[3]}{h}$$
		$$m=\lim_{h \to 0}\frac{2+2h+1+2h+h^2-3}{h}$$
			$$m=\lim_{h \to 0}\frac{h^2+4h}{h}$$
				$$m=\lim_{h \to 0}(h+4)$$
					$$m=4$$
						The slope of the tangent line at the point (1,3) on the curve $f(x)=2x+x^2$ is 4.\
						

Notice that we found the slope of this same curve using the secant method in a previous example. The results happen to be exactly the same in this case, but the First Principles method is more accurate and efficient.				
						
## The Equation of a Tangent
#### The equation of a line is $m=(x-x_1)+y_1$.
Find the equation of the tangent line at point (1,3) on the curve $f(x)=2x+x^2$.

So, we know already that $m=4$ from the previous example. 
	$$y=4(x-1)+3$$
		$$y=4x-4+3$$
			$$y=4x-1$$
				The equation of the tangent line is $y=4x-1$.
				
### Now, find the equation of the tangent line at point (2,3) on the curve $f(x)=2x^2-3x+1$.

1. Find the slope of the tangent line at point (2,3)
#### $$m=\lim_{h \to 0}\frac{f(a+h)-f(a)}{h}$$
$$m=\lim_{h \to 0}\frac{[2(2+h)^2-3(2+h)+1]-2(2)^2-3(2)+1}{h}$$
	$$m=\lim_{h \to 0}\frac{[2(4+4h+h^2)-6-3h+1]-[3]}{h}$$
		$$m=\lim_{h \to 0}\frac{8+8h+2h^2-6-3h+1-3}{h}$$
			$$m=\lim_{h \to 0}\frac{2h^2+5h}{h}$$
				$$m=\lim_{h\to 0}(2h+5)$$
					$$m=5$$
The slope of the tangent line is 5 at point (2,3)

2. Equation of the tangent
	#### $$y=m(x-x_1)+y_1$$
	$$y=5(x-2)+3$$
		$$5x-10+3$$
			$$5x-7$$
The equation of the tangent line at the point (2,3) is $y=5x-7$.
		
							
		




		